done

project/out/Top_level.ml
@@ -39,7 +39,8 @@ let (start : state) =
 let (handle_load_in_new_win_event :
   Browser.win_opener ->
     Browser.win_name ->
-      BrowserIO.url -> Browser.browser -> (state * output_event Prims.list))
+      BrowserIO.url ->
+        Browser.browser -> (state * BrowserIO.output_event Prims.list))
   =
   fun wo ->
     fun wn ->
@@ -52,7 +53,8 @@ let (handle_load_in_new_win_event :
               ((Running r), oes)
 let (handle_load_in_win_event :
   Browser.win_ref ->
-    BrowserIO.url -> Browser.browser -> (state * output_event Prims.list))
+    BrowserIO.url ->
+      Browser.browser -> (state * BrowserIO.output_event Prims.list))
   =
   fun wr ->
     fun u ->
@@ -66,7 +68,9 @@ let (handle_load_in_win_event :
               ((Running r), oes)
         else ((Waiting b), [BrowserIO.UI_error "invalid win_ref"])
 let (handle_close_win_event :
-  Browser.win_ref -> Browser.browser -> (state * output_event Prims.list)) =
+  Browser.win_ref ->
+    Browser.browser -> (state * BrowserIO.output_event Prims.list))
+  =
   fun wr ->
     fun b ->
       if
@@ -81,7 +85,8 @@ let (handle_close_win_event :
 let (handle_input_text_event :
   Browser.win_ref ->
     Prims.nat ->
-      Prims.string -> Browser.browser -> (state * output_event Prims.list))
+      Prims.string ->
+        Browser.browser -> (state * BrowserIO.output_event Prims.list))
   =
   fun wr ->
     fun box_pos ->
@@ -116,7 +121,8 @@ let (handle_input_text_event :
           else ((Waiting b), [BrowserIO.UI_error "invalid win_ref"])
 let (handle_click_button_event :
   Browser.win_ref ->
-    Prims.nat -> Browser.browser -> (state * output_event Prims.list))
+    Prims.nat ->
+      Browser.browser -> (state * BrowserIO.output_event Prims.list))
   =
   fun wr ->
     fun but_pos ->
@@ -168,3 +174,275 @@ let (get_ready_exprs :
             let b' = Browser.page_update w.Browser.win_page p' b in
             ((FStar_List_Tot_Base.map task pes_ready), b')
       else ([], b)
+let (handle_network_response_event :
+  BrowserIO.net_connection ->
+    BrowserIO.resp ->
+      Browser.browser -> (state * BrowserIO.output_event Prims.list))
+  =
+  fun nc ->
+    fun resp ->
+      fun b ->
+        let uu___ = nc in
+        match uu___ with
+        | (d, n) ->
+            (match Browser.net_connection_domain_nth d n b with
+             | FStar_Pervasives_Native.None -> ((Waiting b), [])
+             | FStar_Pervasives_Native.Some (uri, dst) ->
+                 let b' = Browser.net_connection_domain_remove_nth d n b in
+                 let b'1 = Browser.upd_cookies d uri resp b' in
+                 (match (dst, (resp.BrowserIO.resp_body)) with
+                  | (Browser.Xhr_dst (pr, v), BrowserIO.Script_file e) ->
+                      (match Browser.page_win pr b'1 with
+                       | FStar_Pervasives_Native.Some w ->
+                           let wr = w in
+                           let t =
+                             {
+                               Browser.task_win = wr;
+                               Browser.task_expr =
+                                 (BrowserIO.Apply
+                                    ((BrowserIO.X (Browser.R v)),
+                                      (BrowserIO.X
+                                         (Browser.R (Browser.Code_value e)))))
+                             } in
+                           let r =
+                             { running_state = b'1; running_task_queue = [t]
+                             } in
+                           ((Running r), [])
+                       | FStar_Pervasives_Native.None -> ((Waiting b), []))
+                  | (Browser.Doc_dst wr, BrowserIO.Html_file docs) ->
+                      if
+                        (Browser.win_valid wr b'1) &&
+                          (Browser.page_valid
+                             (Browser.win_assoc_valid wr b'1).Browser.win_page
+                             b'1)
+                      then
+                        let uw = Browser.win_to_user_window wr b'1 in
+                        let w = Browser.win_assoc_valid wr b'1 in
+                        let b'2 = Browser.page_remove w.Browser.win_page b'1 in
+                        let nd_ref =
+                          if
+                            (FStar_List_Tot_Base.length
+                               b'2.Browser.browser_nodes)
+                              >= Prims.int_one
+                          then
+                            FStar_Pervasives_Native.fst
+                              (FStar_List_Tot_Base.last
+                                 b'2.Browser.browser_nodes)
+                          else Prims.int_zero in
+                        let uu___1 =
+                          Browser.build_node_tree
+                            (BrowserIO.Divi
+                               (FStar_Pervasives_Native.None, docs)) nd_ref in
+                        (match uu___1 with
+                         | (dr, node_ext) ->
+                             let new_nodes =
+                               FStar_List_Tot_Base.op_At
+                                 b'2.Browser.browser_nodes node_ext in
+                             let b'3 =
+                               if Browser.b_node_pred new_nodes
+                               then
+                                 {
+                                   Browser.browser_windows =
+                                     (b'2.Browser.browser_windows);
+                                   Browser.browser_pages =
+                                     (b'2.Browser.browser_pages);
+                                   Browser.browser_nodes = new_nodes;
+                                   Browser.browser_environments =
+                                     (b'2.Browser.browser_environments);
+                                   Browser.browser_cookies =
+                                     (b'2.Browser.browser_cookies);
+                                   Browser.browser_connections =
+                                     (b'2.Browser.browser_connections)
+                                 }
+                               else failwith "b_node_pred is not satisfied" in
+                             let uu___2 =
+                               Browser.build_win w.Browser.win_name
+                                 (BrowserIO.Http_url (d, uri))
+                                 w.Browser.win_opener
+                                 (FStar_Pervasives_Native.Some dr) b'3 in
+                             (match uu___2 with
+                              | (w', b'4) ->
+                                  let b'5 = Browser.win_update wr w' b'4 in
+                                  let rd_opt =
+                                    Browser.render_page w'.Browser.win_page
+                                      b'4 in
+                                  let oe =
+                                    BrowserIO.UI_page_loaded_event
+                                      (uw, (BrowserIO.Http_url (d, uri)),
+                                        rd_opt) in
+                                  let uu___3 =
+                                    Browser.process_node_scripts
+                                      w'.Browser.win_page dr b'5 in
+                                  (match uu___3 with
+                                   | (b'6, oes1, ts) ->
+                                       let r =
+                                         {
+                                           running_state = b'6;
+                                           running_task_queue = ts
+                                         } in
+                                       ((Running r),
+                                         (FStar_List_Tot_Base.op_At [oe] oes1)))))
+                      else ((Waiting b'1), [])
+                  | (Browser.Doc_dst wr, uu___1) ->
+                      if
+                        (Browser.win_valid wr b'1) &&
+                          (Browser.page_valid
+                             (Browser.win_assoc_valid wr b'1).Browser.win_page
+                             b'1)
+                      then
+                        let uw = Browser.win_to_user_window wr b'1 in
+                        let w = Browser.win_assoc_valid wr b'1 in
+                        let b'3 = Browser.page_remove w.Browser.win_page b'1 in
+                        let uu___2 =
+                          Browser.build_win w.Browser.win_name
+                            (BrowserIO.Http_url (d, uri))
+                            w.Browser.win_opener FStar_Pervasives_Native.None
+                            b'3 in
+                        (match uu___2 with
+                         | (w', b'4) ->
+                             let b'5 = Browser.win_update wr w' b'4 in
+                             let rd_opt =
+                               Browser.render_page w'.Browser.win_page b'5 in
+                             let oe =
+                               BrowserIO.UI_page_loaded_event
+                                 (uw, (BrowserIO.Http_url (d, uri)), rd_opt) in
+                             ((Waiting b'5), [oe]))
+                      else ((Waiting b'1), [])
+                  | (Browser.Script_dst (pr, dr), BrowserIO.Script_file e) ->
+                      if Browser.page_valid pr b'1
+                      then
+                        (match Browser.page_win pr b'1 with
+                         | FStar_Pervasives_Native.Some w ->
+                             let wr = w in
+                             let p = Browser.page_assoc_valid pr b'1 in
+                             let q = p.Browser.page_script_queue in
+                             let q' =
+                               let upd p1 =
+                                 match p1 with
+                                 | Browser.Unknown_expr dr1 ->
+                                     if dr1 = dr
+                                     then
+                                       Browser.Known_expr
+                                         (Browser.to_inner_expr e)
+                                     else p1
+                                 | uu___1 -> p1 in
+                               FStar_List_Tot_Base.map upd q in
+                             let p' =
+                               {
+                                 Browser.page_location =
+                                   (p.Browser.page_location);
+                                 Browser.page_document =
+                                   (p.Browser.page_document);
+                                 Browser.page_environment =
+                                   (p.Browser.page_environment);
+                                 Browser.page_script_queue = q'
+                               } in
+                             let b'2 = Browser.page_update pr p' b'1 in
+                             let uu___1 = get_ready_exprs wr b'2 in
+                             (match uu___1 with
+                              | (ts, b'3) ->
+                                  let r =
+                                    {
+                                      running_state = b'3;
+                                      running_task_queue = ts
+                                    } in
+                                  ((Running r), []))
+                         | FStar_Pervasives_Native.None ->
+                             ((Waiting b'1), []))
+                      else failwith "page not in browser"
+                  | uu___1 -> ((Waiting b'1), [])))
+let (receive :
+  BrowserIO.input_event ->
+    waiting -> (state * BrowserIO.output_event Prims.list))
+  =
+  fun ie ->
+    fun w ->
+      match ie with
+      | BrowserIO.User_load_in_new_win_event u ->
+          handle_load_in_new_win_event Browser.No_opener Browser.No_name u w
+      | BrowserIO.User_load_in_win_event (uw, u) ->
+          (match Browser.win_from_user_window uw w with
+           | FStar_Pervasives_Native.None -> ((Waiting w), [])
+           | FStar_Pervasives_Native.Some wr ->
+               handle_load_in_win_event wr u w)
+      | BrowserIO.User_link_to_new_win_event (uw, u) ->
+          let wo =
+            match Browser.win_from_user_window uw w with
+            | FStar_Pervasives_Native.None -> Browser.No_opener
+            | FStar_Pervasives_Native.Some wr -> Browser.Win_opener wr in
+          handle_load_in_new_win_event wo Browser.No_name u w
+      | BrowserIO.User_link_to_named_win_event (uw, str, u) ->
+          let wo =
+            match Browser.win_from_user_window uw w with
+            | FStar_Pervasives_Native.None -> Browser.No_opener
+            | FStar_Pervasives_Native.Some wr -> Browser.Win_opener wr in
+          (match Browser.win_from_win_name str w with
+           | FStar_Pervasives_Native.None ->
+               handle_load_in_new_win_event wo (Browser.Str_name str) u w
+           | FStar_Pervasives_Native.Some wr ->
+               handle_load_in_win_event wr u w)
+      | BrowserIO.User_close_win_event uw ->
+          (match Browser.win_from_user_window uw w with
+           | FStar_Pervasives_Native.None -> ((Waiting w), [])
+           | FStar_Pervasives_Native.Some wr -> handle_close_win_event wr w)
+      | BrowserIO.User_input_text_event ((uw, box_pos), str) ->
+          (match Browser.win_from_user_window uw w with
+           | FStar_Pervasives_Native.None -> ((Waiting w), [])
+           | FStar_Pervasives_Native.Some wr ->
+               handle_input_text_event wr box_pos str w)
+      | BrowserIO.User_click_button_event (uw, but_pos) ->
+          (match Browser.win_from_user_window uw w with
+           | FStar_Pervasives_Native.None -> ((Waiting w), [])
+           | FStar_Pervasives_Native.Some wr ->
+               handle_click_button_event wr but_pos w)
+      | BrowserIO.Network_response_event (nr, resp) ->
+          handle_network_response_event nr resp w
+let (continue : running -> (state * BrowserIO.output_event Prims.list)) =
+  fun r ->
+    let current t = Browser.win_valid t.Browser.task_win r.running_state in
+    match r.running_task_queue with
+    | [] -> ((Waiting (r.running_state)), [])
+    | t::ts ->
+        if Prims.op_Negation (current t)
+        then
+          let r' =
+            { running_state = (r.running_state); running_task_queue = ts } in
+          ((Running r'), [])
+        else
+          (match t.Browser.task_expr with
+           | BrowserIO.X (Browser.R (Browser.Error msg)) ->
+               let r' =
+                 { running_state = (r.running_state); running_task_queue = ts
+                 } in
+               ((Running r'), [BrowserIO.UI_error msg])
+           | BrowserIO.X (Browser.R uu___1) ->
+               let r' =
+                 { running_state = (r.running_state); running_task_queue = ts
+                 } in
+               ((Running r'), [])
+           | uu___1 ->
+               let b = r.running_state in
+               let w = Browser.win_assoc_valid t.Browser.task_win b in
+               if Browser.page_valid w.Browser.win_page b
+               then
+                 let p = Browser.page_assoc_valid w.Browser.win_page b in
+                 let ctx =
+                   {
+                     Browser.context_win = (t.Browser.task_win);
+                     Browser.context_act = (p.Browser.page_environment)
+                   } in
+                 let uu___2 = Browser.step_expr ctx b t.Browser.task_expr in
+                 (match uu___2 with
+                  | (b', e', oes, ts') ->
+                      let r' =
+                        {
+                          running_state = b';
+                          running_task_queue =
+                            (FStar_List_Tot_Base.op_At
+                               ({
+                                  Browser.task_win = (t.Browser.task_win);
+                                  Browser.task_expr = e'
+                                } :: ts) ts')
+                        } in
+                      ((Running r'), oes))
+               else failwith "page not valid")
