project/Top_level.fst
@@ -4,37 +4,9 @@ open BrowserIO
 open Assumed
 open Browser
 open FStar.List.Tot.Base
+open FStar.All
 
 (** {3 Top-level browser functionality} *)
-
-  (** The type of a browser waiting for input. *)
-  type waiting = browser
-
-  (** The type of a browser in the middle of processing the current input. *)
-  type running = {
-    running_state: browser;
-    running_task_queue: list task;
-  }
-
- 
-  type input_event = BrowserIO.input_event
-  type output_event = BrowserIO.output_event
-
-  (** The type of a browser state, in general. *)
-  type state =
-    | Waiting of waiting
-    | Running of running
-
-  (** The initial configuration of a browser. *)
-  let start: state =
-    Waiting ({
-        browser_windows = [];
-        browser_pages = [];
-        browser_nodes = [];
-        browser_environments = [];
-        browser_cookies = [];
-        browser_connections = [];
-    })
 
   (** Handling a [User_load_in_new_win_event]. *)
   let handle_load_in_new_win_event
@@ -135,193 +107,220 @@ open FStar.List.Tot.Base
     ([],b)
 
 
-  // (** Handling a [Network_response_event]. *)
-  // let handle_network_response_event
-  //   (Net_connection(d, n): net_connection) (resp: resp) (b: browser)
-  // : state * list output_event =
-  //   begin match net_connection_domain_nth d n b with
-  //   | None ->
-  //       (Waiting(b), [])
-  //   | Some((uri, dst)) ->
-  //       let b' = net_connection_domain_remove_nth d n b in
-  //       let b'1 = upd_cookies d uri resp b' in
-  //       begin match (dst, resp.resp_body) with
+  (** Handling a [Network_response_event]. *)
+  let handle_network_response_event
+    (nc: net_connection) (resp: resp) (b: browser)
+  : All (state * list output_event) 
+    (requires (fun h0 ->  True))
+    (ensures (fun h0 r h1 -> True))
+  =
+    let (d,n) = nc in 
+    begin match net_connection_domain_nth d n b with
+    | None ->
+      (Waiting(b), [])
+    | Some((uri, dst)) ->
+        let b' = net_connection_domain_remove_nth d n b in
+        let b'1 = upd_cookies d uri resp b' in
+        begin match (dst, resp.resp_body) with
 
-  //       | (Xhr_dst(pr, v), Script_file(e)) when page_win pr b'1 <> None ->
-  //           let wr =
-  //             begin match page_win pr b'1 with
-  //             | Some(wr) -> wr
-  //             | None -> assert false
-  //             end
-  //           in
-  //           let t = {
-  //             task_win = wr;
-  //             task_expr = Apply(X(R(v)), X(R(Code_value(e))));
-  //           } in
-  //           let r = {
-  //             running_state = b'1;
-  //             running_task_queue = [ t ];
-  //           } in
-  //           (Running(r), [])
+        | (Xhr_dst(pr, v), Script_file(e))  -> 
+            begin match page_win pr b'1 with
+              | Some(w) -> 
+                let wr = w   
+              in
+              let t = {
+                task_win = wr;
+                task_expr = Apply(X(R(v)), X(R(Code_value(e))));
+              } in
+              let r = {
+                running_state = b'1;
+                running_task_queue = [ t ];
+              } in
+              (Running(r), [])
 
-  //       | (Doc_dst(wr), Html_file(docs)) when win_valid wr b'1 ->
-  //           let uw = win_to_user_window wr b'1 in
-  //           let w = win_assoc_valid wr b'1 in
-  //           let b'2 = page_remove w.win_page b'1 in
-  //           let (dr, node_ext) = build_node_tree (Div(None, docs)) in
-  //           let b'3 = {
-  //             b'2 with
-  //             browser_nodes = b'2.browser_nodes @ node_ext
-  //           } in
-  //           let (w', b'4) =
-  //             build_win
-  //               w.win_name (Http_url(d, uri)) w.win_opener (Some(dr)) b'3
-  //           in
-  //           let b'5 = win_update wr w' b'4 in
-  //           let rd_opt = render_page w'.win_page b'4 in
-  //           let oe = UI_page_loaded_event(uw, Http_url(d, uri), rd_opt) in
-  //           let (b'6, oes1, ts) = process_node_scripts w'.win_page dr b'5 in
-  //           let r = {
-  //             running_state = b'6;
-  //             running_task_queue = ts;
-  //           } in
-  //           (Running(r), [ oe ] @ oes1)
+              | None -> (Waiting(b), [])
+              end
+           
 
-  //       | (Doc_dst(wr), _) when win_valid wr b'1 ->
-  //           let uw = win_to_user_window wr b'1 in
-  //           let w = win_assoc_valid wr b'1 in
-  //           let b'3 = page_remove w.win_page b'1 in
-  //           let (w', b'4) =
-  //             build_win w.win_name (Http_url(d, uri)) w.win_opener None b'3
-  //           in
-  //           let b'5 = win_update wr w' b'4 in
-  //           let rd_opt = render_page w'.win_page b'5 in
-  //           let oe = UI_page_loaded_event(uw, Http_url(d, uri), rd_opt) in
-  //           (Waiting({ waiting_state = b'5 }), [ oe ])
+        | (Doc_dst(wr), Html_file(docs)) -> if (win_valid wr b'1 && page_valid (win_assoc_valid wr b'1).win_page b'1 ) then
+            let uw = win_to_user_window wr b'1 in
+            let w = win_assoc_valid wr b'1 in
+            let b'2 = page_remove w.win_page b'1 in
+            let nd_ref= if length b'2.browser_nodes >= 1 then (fst (last b'2.browser_nodes)) else 0 in
+            let (dr, node_ext) = build_node_tree (Divi(None, docs)) (nd_ref) in
+            let new_nodes = b'2.browser_nodes @ node_ext in 
+            let b'3 = 
+              if (b_node_pred new_nodes) then
+              {b'2 with
+              browser_nodes = new_nodes}
+              else 
+              failwith "b_node_pred is not satisfied"
+            in
+            let (w', b'4) =
+              build_win
+                w.win_name (Http_url(d, uri)) w.win_opener (Some(dr)) b'3
+            in
+            let b'5 = win_update wr w' b'4 in
+            let rd_opt = render_page w'.win_page b'4 in
+            let oe = UI_page_loaded_event(uw, Http_url(d, uri), rd_opt) in
+            let (b'6, oes1, ts) = process_node_scripts w'.win_page dr b'5 in
+            let r = {
+              running_state = b'6;
+              running_task_queue = ts;
+            } in
+            (Running(r), [ oe ] @ oes1)
 
-  //       | (Script_dst(pr, dr), Script_file(e)) when page_win pr b'1 <> None ->
-  //           let wr =
-  //             begin match page_win pr b'1 with
-  //             | Some(wr) -> wr
-  //             | None -> assert false
-  //             end
-  //           in
-  //           let p = page_assoc_valid pr b'1 in
-  //           let q = p.page_script_queue in
-  //           let q' =
-  //             let upd p =
-  //               begin match p with
-  //               | Unknown_expr(dr1) when dr1 = dr -> Known_expr(to_inner_expr e)
-  //               | _ -> p
-  //               end
-  //             in
-  //             List.map upd q
-  //           in
-  //           let p' = { p with page_script_queue = q' } in
-  //           let b'2 = page_update pr p' b'1 in
-  //           let (ts, b'3) = get_ready_exprs wr b'2 in
-  //           let r = {
-  //             running_state = b'3;
-  //             running_task_queue = ts;
-  //           } in
-  //           (Running(r), [])
+            else (Waiting(b'1), [])
 
-  //       | _ ->
-  //         (Waiting({ waiting_state = b'1 }), [])
+        | (Doc_dst(wr), _)  -> if (win_valid wr b'1 && page_valid (win_assoc_valid wr b'1).win_page b'1 ) then
+            let uw = win_to_user_window wr b'1 in
+            let w = win_assoc_valid wr b'1 in
+            let b'3 = page_remove w.win_page b'1 in
+            let (w', b'4) =
+              build_win w.win_name (Http_url(d, uri)) w.win_opener None b'3
+            in
+            let b'5 = win_update wr w' b'4 in
+            let rd_opt = render_page w'.win_page b'5 in
+            let oe = UI_page_loaded_event(uw, Http_url(d, uri), rd_opt) in
+            (Waiting(b'5), [ oe ])
 
-  //       end
-  //   end
+            else (Waiting(b'1), [])
 
-  // (** Respond to an incoming event. *)
-  // let receive (ie: input_event) (w: waiting)
-  // : state * list output_event=
-  //   begin match ie with
+        | (Script_dst(pr, dr), Script_file(e)) ->
+              if (page_valid pr b'1) then
+              begin match page_win pr b'1 with
+              | Some(w) -> 
+                let wr = w
+                  in
+                let p = page_assoc_valid pr b'1 in
+                let q = p.page_script_queue in
+                let q' =
+                  let upd p =
+                    begin match p with
+                    | Unknown_expr(dr1)  -> if dr1 = dr then Known_expr(to_inner_expr e)
+                    else p
+                    | _ -> p
+                    end
+                  in
+                  map upd q
+                in
+                let p' = { p with page_script_queue = q' } in
+                let b'2 = page_update pr p' b'1 in
+                let (ts, b'3) = get_ready_exprs wr b'2 in
+                let r = {
+                  running_state = b'3;
+                  running_task_queue = ts;
+                } in
+                (Running(r), [])
 
-  //   | User_load_in_new_win_event(u) ->
-  //       handle_load_in_new_win_event No_opener No_name u w.waiting_state
+              | None -> (Waiting(b'1), [])
+              end
+              else failwith "page not in browser"
+            
 
-  //   | User_load_in_win_event(uw, u) ->
-  //       begin match win_from_user_window uw w.waiting_state with
-  //       | None -> (Waiting(w), [])
-  //       | Some(wr) -> handle_load_in_win_event wr u w.waiting_state
-  //       end
+        | _ ->
+          (Waiting(b'1), [])
 
-  //   | User_link_to_new_win_event(uw, u) ->
-  //       let wo =
-  //         begin match win_from_user_window uw w.waiting_state with
-  //         | None -> No_opener
-  //         | Some(wr) -> Win_opener(wr)
-  //         end
-  //       in
-  //       handle_load_in_new_win_event wo No_name u w.waiting_state
+        end
+    end
 
-  //   | User_link_to_named_win_event(uw, str, u) ->
-  //       let wo =
-  //         begin match win_from_user_window uw w.waiting_state with
-  //         | None -> No_opener
-  //         | Some(wr) -> Win_opener(wr)
-  //         end
-  //       in
-  //       begin match win_from_win_name str w.waiting_state with
-  //       | None ->
-  //           handle_load_in_new_win_event wo (Str_name(str)) u w.waiting_state
-  //       | Some(wr) ->
-  //           handle_load_in_win_event wr u w.waiting_state
-  //       end
+  (** Respond to an incoming event. *)
+  let receive (ie: input_event) (w: waiting) =
+    begin match ie with
 
-  //   | User_close_win_event(uw) ->
-  //       begin match win_from_user_window uw w.waiting_state with
-  //       | None -> (Waiting(w), [])
-  //       | Some(wr) -> handle_close_win_event wr w.waiting_state
-  //       end
+    | User_load_in_new_win_event(u) ->
+        handle_load_in_new_win_event No_opener No_name u w
 
-  //   | User_input_text_event(User_textbox(uw, box_pos), str, _) ->
-  //       begin match win_from_user_window uw w.waiting_state with
-  //       | None -> (Waiting(w), [])
-  //       | Some(wr) -> handle_input_text_event wr box_pos str w.waiting_state
-  //       end
+    | User_load_in_win_event(uw, u) ->
+        begin match win_from_user_window uw w with
+        | None -> (Waiting(w), [])
+        | Some(wr) -> handle_load_in_win_event wr u w
+        end
 
-  //   | User_click_button_event(User_button(uw, but_pos)) ->
-  //       begin match win_from_user_window uw w.waiting_state with
-  //       | None -> (Waiting(w), [])
-  //       | Some(wr) -> handle_click_button_event wr but_pos w.waiting_state
-  //       end
+    | User_link_to_new_win_event(uw, u) ->
+        let wo =
+          begin match win_from_user_window uw w with
+          | None -> No_opener
+          | Some(wr) -> Win_opener(wr)
+          end
+        in
+        handle_load_in_new_win_event wo No_name u w
 
-  //   | Network_response_event(nr, resp) ->
-  //       handle_network_response_event nr resp w.waiting_state
+    | User_link_to_named_win_event(uw, str, u) ->
+        let wo =
+          begin match win_from_user_window uw w with
+          | None -> No_opener
+          | Some(wr) -> Win_opener(wr)
+          end
+        in
+        begin match win_from_win_name str w with
+        | None ->
+            handle_load_in_new_win_event wo (Str_name(str)) u w
+        | Some(wr) ->
+            handle_load_in_win_event wr u w
+        end
 
-  //   end
+    | User_close_win_event(uw) ->
+        begin match win_from_user_window uw w with
+        | None -> (Waiting(w), [])
+        | Some(wr) -> handle_close_win_event wr w
+        end
 
-  // (** Advance the browser state one step. *)
-  // let continue (r: running)
-  // : state * list output_event =
-  //   let current t = win_valid t.task_win r.running_state in
-  //   begin match r.running_task_queue with
-  //   | [] ->
-  //       (Waiting({ waiting_state = r.running_state}), [])
-  //   | t :: ts when not (current t) ->
-  //       let r' = { r with running_task_queue = ts } in
-  //       (Running(r'), [])
-  //   | { task_expr = X(R(Error(msg))) } :: ts ->
-  //       let r' = { r with running_task_queue = ts } in
-  //       (Running(r'), [ UI_error(msg) ])
-  //   | { task_expr = X(R(_)) } :: ts ->
-  //       let r' = { r with running_task_queue = ts } in
-  //       (Running(r'), [])
-  //   | t :: ts -> (* the task is current and not finished *)
-  //       let b = r.running_state in
-  //       let w = win_assoc_valid t.task_win b in
-  //       let p = page_assoc_valid w.win_page b in
-  //       let ctx = {
-  //         context_win = t.task_win;
-  //         context_act = p.page_environment;
-  //       } in
-  //       let (b', e', oes, ts') = step_expr ctx b t.task_expr in
-  //       let r' = {
-  //         running_state = b';
-  //         running_task_queue = { t with task_expr = e' } :: ts @ ts';
-  //       } in
-  //       (Running(r'), oes)
-  //   end
+    | User_input_text_event((uw, box_pos), str) ->
+        begin match win_from_user_window uw w with
+        | None -> (Waiting(w), [])
+        | Some(wr) -> handle_input_text_event wr box_pos str w
+        end
+
+    | User_click_button_event((uw, but_pos)) ->
+        begin match win_from_user_window uw w with
+        | None -> (Waiting(w), [])
+        | Some(wr) -> handle_click_button_event wr but_pos w
+        end
+
+    | Network_response_event(nr, resp) ->
+        handle_network_response_event nr resp w
+
+    end
+
+  (** Advance the browser state one step. *)
+  let continue (r: running) =
+
+    let current t = win_valid t.task_win r.running_state in
+    begin match r.running_task_queue with
+    | [] ->
+        (Waiting(r.running_state), [])
+    | t :: ts -> 
+      if (not(current t)) then 
+        let r' = { r with running_task_queue = ts } in
+        (Running(r'), [])
+      else 
+        begin match t.task_expr with 
+        | X(R(Error(msg))) ->
+          let r' = { r with running_task_queue = ts } in
+          (Running(r'), [ UI_error(msg) ])
+        | X(R(_)) ->
+          let r' = { r with running_task_queue = ts } in
+          (Running(r'), [])
+        | _ -> (* the task is current and not finished *)
+        let b = r.running_state in
+        let w = win_assoc_valid t.task_win b in
+        if (page_valid w.win_page b) then
+        let p = page_assoc_valid w.win_page b in
+        let ctx = {
+          context_win = t.task_win;
+          context_act = p.page_environment;
+        } in
+        let (b', e', oes, ts') = step_expr ctx b t.task_expr in
+        let r' = {
+          running_state = b';
+          running_task_queue = { t with task_expr = e' } :: ts @ ts';
+        } in
+        (Running(r'), oes)
+        
+        else failwith "page not valid"
+
+        end
+    end
 
 
