project/Top_level.fsti
@@ -1,0 +1,46 @@
+module Top_level
+
+open BrowserIO
+open Assumed
+open Browser
+
+(** The definition of a reactive system. *)
+
+ (** The type of a browser waiting for input. *)
+  type waiting = browser
+
+  (** The type of a browser in the middle of processing the current input. *)
+  type running = {
+    running_state: browser;
+    running_task_queue: list task;
+  }
+
+ 
+  type input_event = BrowserIO.input_event
+  type output_event = BrowserIO.output_event
+
+  (** The type of a browser state, in general. *)
+  type state =
+    | Waiting of waiting
+    | Running of running
+
+  (** The initial configuration of a browser. *)
+  let start: state =
+    Waiting ({
+        browser_windows = [];
+        browser_pages = [];
+        browser_nodes = [];
+        browser_environments = [];
+        browser_cookies = [];
+        browser_connections = [];
+    })
+
+  val receive: input_event -> waiting -> 
+    All (state * list output_event) 
+        (requires (fun h0 ->  True))
+        (ensures (fun h0 r h1 -> True))
+
+  val continue: running -> 
+    All (state * list (output_event))
+        (requires (fun h0 ->  True))
+        (ensures (fun h0 r h1 -> True))
